stage0/stdlib/Init/Core.c
@@ -57,12 +57,12 @@ static lean_object* l_myMacro____x40_Init_Core___hyg_1147____closed__6;
 static lean_object* l_term___u2248_____closed__7;
 uint8_t l_decidableOfDecidableOfEq___rarg(uint8_t, lean_object*);
 static lean_object* l_term___x21_x3d_____closed__5;
-static lean_object* l_myMacro____x40_Init_Core___hyg_1977____closed__3;
 lean_object* l_Quot_indep(lean_object*, lean_object*, lean_object*);
 lean_object* l_Eq_ndrecOn___rarg(lean_object*);
 static lean_object* l_term_x7b_x7d___closed__4;
 static lean_object* l_term___x21_x3d_____closed__2;
 static lean_object* l_term___u2260_____closed__1;
+static lean_object* l_myMacro____x40_Init_Core___hyg_1981____closed__3;
 lean_object* l_Quot_liftOn___rarg(lean_object*, lean_object*, lean_object*);
 lean_object* l_instDecidableEqProd_match__2(lean_object*, lean_object*, lean_object*);
 lean_object* l_Eq_mpr___rarg___boxed(lean_object*);
@@ -107,23 +107,22 @@ lean_object* l_instHasEquiv(lean_object*, lean_object*);
 lean_object* l_Quotient_lift_u2082___rarg(lean_object*, lean_object*, lean_object*, lean_object*);
 static lean_object* l_term___u2194_____closed__2;
 lean_object* l_Task_bind___boxed(lean_object*, lean_object*, lean_object*, lean_object*, lean_object*);
-static lean_object* l_myMacro____x40_Init_Core___hyg_1977____closed__4;
 lean_object* lean_thunk_pure(lean_object*);
 lean_object* l_term___u2260__;
 lean_object* l_decidableOfDecidableOfEq___rarg___boxed(lean_object*, lean_object*);
 lean_object* l_toBoolUsing___rarg___boxed(lean_object*);
+static lean_object* l_myMacro____x40_Init_Core___hyg_1981____closed__2;
 lean_object* l_strictOr___boxed(lean_object*, lean_object*);
 lean_object* l_Quotient_recOnSubsingleton_u2082___boxed(lean_object*, lean_object*, lean_object*, lean_object*, lean_object*, lean_object*);
 lean_object* l_Subtype_instDecidableEqSubtype___rarg(lean_object*, lean_object*, lean_object*);
 static lean_object* l_term___x3c_x2d_x3e_____closed__6;
-static lean_object* l_myMacro____x40_Init_Core___hyg_1977____closed__6;
 static lean_object* l_myMacro____x40_Init_Core___hyg_175____closed__11;
 lean_object* l_Quotient_mk___boxed(lean_object*, lean_object*);
 lean_object* l_instDecidableEqQuotient___boxed(lean_object*, lean_object*);
 lean_object* l_instInhabitedTask(lean_object*);
+static lean_object* l_myMacro____x40_Init_Core___hyg_1981____closed__1;
 static lean_object* l_myMacro____x40_Init_Core___hyg_175____closed__12;
 lean_object* l_Thunk_bind___rarg___lambda__1___boxed(lean_object*, lean_object*, lean_object*);
-static lean_object* l_myMacro____x40_Init_Core___hyg_1576____closed__3;
 lean_object* l_instDecidableDite___rarg(uint8_t, lean_object*, lean_object*);
 static lean_object* l_term___u2260_____closed__6;
 lean_object* l_Eq_mpr(lean_object*, lean_object*, lean_object*);
@@ -131,6 +130,7 @@ lean_object* l_Quot_recOn___rarg(lean_object*, lean_object*, lean_object*);
 lean_object* l_Thunk_get___boxed(lean_object*, lean_object*);
 static lean_object* l_term___u2194_____closed__4;
 lean_object* l_Quot_recOnSubsingleton(lean_object*, lean_object*, lean_object*, lean_object*);
+static lean_object* l_myMacro____x40_Init_Core___hyg_1580____closed__3;
 lean_object* l_Lean_reduceNat(lean_object*);
 lean_object* l_Squash_lift___rarg(lean_object*, lean_object*);
 lean_object* l_Sum_inhabitedLeft___rarg(lean_object*);
@@ -141,8 +141,8 @@ lean_object* l_Quot_hrecOn(lean_object*, lean_object*, lean_object*);
 lean_object* l_myMacro____x40_Init_Core___hyg_1147_(lean_object*, lean_object*, lean_object*);
 lean_object* l_myMacro____x40_Init_Core___hyg_907_(lean_object*, lean_object*, lean_object*);
 lean_object* l_myMacro____x40_Init_Core___hyg_414_(lean_object*, lean_object*, lean_object*);
-lean_object* l_myMacro____x40_Init_Core___hyg_1576_(lean_object*, lean_object*, lean_object*);
-lean_object* l_myMacro____x40_Init_Core___hyg_1977_(lean_object*, lean_object*, lean_object*);
+lean_object* l_myMacro____x40_Init_Core___hyg_1580_(lean_object*, lean_object*, lean_object*);
+lean_object* l_myMacro____x40_Init_Core___hyg_1981_(lean_object*, lean_object*, lean_object*);
 lean_object* l_myMacro____x40_Init_Core___hyg_1282_(lean_object*, lean_object*, lean_object*);
 lean_object* l_myMacro____x40_Init_Core___hyg_175_(lean_object*, lean_object*, lean_object*);
 static lean_object* l_myMacro____x40_Init_Core___hyg_1147____closed__7;
@@ -160,15 +160,15 @@ lean_object* l_instInhabitedPNonScalar;
 static lean_object* l_term___x3c_x2d_x3e_____closed__11;
 lean_object* l_instDecidableEqQuotient(lean_object*, lean_object*);
 static lean_object* l_myMacro____x40_Init_Core___hyg_1147____closed__2;
+static lean_object* l_myMacro____x40_Init_Core___hyg_1981____closed__6;
 lean_object* lean_task_map(lean_object*, lean_object*, lean_object*);
 lean_object* l_instDecidableEqProd_match__2___rarg(lean_object*, lean_object*);
-static lean_object* l_myMacro____x40_Init_Core___hyg_1977____closed__2;
-static lean_object* l_myMacro____x40_Init_Core___hyg_1977____closed__1;
 lean_object* l_instInhabitedProp;
 lean_object* l_flip___rarg(lean_object*, lean_object*, lean_object*);
 lean_object* l_Quotient_hrecOn___boxed(lean_object*, lean_object*, lean_object*);
 static lean_object* l_myMacro____x40_Init_Core___hyg_1147____closed__5;
 lean_object* l_Quotient_rec(lean_object*, lean_object*, lean_object*);
+static lean_object* l_myMacro____x40_Init_Core___hyg_1981____closed__4;
 lean_object* l_Quotient_liftOn_u2082___boxed(lean_object*, lean_object*, lean_object*, lean_object*, lean_object*);
 static lean_object* l_unexpand____x40_Init_Core___hyg_1271____closed__1;
 lean_object* l_instInhabitedNonScalar;
@@ -177,8 +177,8 @@ lean_object* l_unexpand____x40_Init_Core___hyg_1132_(lean_object*, lean_object*)
 lean_object* l_unexpand____x40_Init_Core___hyg_890_(lean_object*, lean_object*);
 lean_object* l_unexpand____x40_Init_Core___hyg_397_(lean_object*, lean_object*);
 lean_object* l_unexpand____x40_Init_Core___hyg_158_(lean_object*, lean_object*);
-lean_object* l_unexpand____x40_Init_Core___hyg_1960_(lean_object*, lean_object*);
-lean_object* l_unexpand____x40_Init_Core___hyg_1559_(lean_object*, lean_object*);
+lean_object* l_unexpand____x40_Init_Core___hyg_1964_(lean_object*, lean_object*);
+lean_object* l_unexpand____x40_Init_Core___hyg_1563_(lean_object*, lean_object*);
 static lean_object* l_myMacro____x40_Init_Core___hyg_175____closed__2;
 lean_object* l_instDecidableIff(lean_object*, lean_object*);
 uint8_t l_instDecidableIff___rarg(uint8_t, uint8_t);
@@ -210,6 +210,7 @@ static lean_object* l_myMacro____x40_Init_Core___hyg_907____closed__9;
 lean_object* l_instBEqProd___rarg(lean_object*, lean_object*, lean_object*, lean_object*);
 static lean_object* l_term_x7b_x7d___closed__5;
 lean_object* l_Lean_addMacroScope(lean_object*, lean_object*, lean_object*);
+static lean_object* l_myMacro____x40_Init_Core___hyg_1580____closed__5;
 lean_object* l_Squash_lift(lean_object*, lean_object*, lean_object*);
 static lean_object* l_term_x7b_x7d___closed__7;
 static lean_object* l_term_u2205___closed__2;
@@ -239,7 +240,6 @@ static lean_object* l_myMacro____x40_Init_Core___hyg_175____closed__6;
 lean_object* l_Thunk_bind___rarg(lean_object*, lean_object*);
 uint8_t l_bne___rarg(lean_object*, lean_object*, lean_object*);
 static lean_object* l_myMacro____x40_Init_Core___hyg_907____closed__4;
-static lean_object* l_myMacro____x40_Init_Core___hyg_1576____closed__5;
 static lean_object* l_myMacro____x40_Init_Core___hyg_175____closed__17;
 lean_object* l_instDecidableEqSum(lean_object*, lean_object*);
 lean_object* l_Subtype_instInhabitedSubtype(lean_object*, lean_object*);
@@ -259,14 +259,12 @@ lean_object* l_Quot_liftOn(lean_object*, lean_object*, lean_object*);
 static lean_object* l_term___x3c_x2d_x3e_____closed__8;
 static lean_object* l_term___u2194_____closed__6;
 lean_object* l_instDecidableDite___rarg___boxed(lean_object*, lean_object*, lean_object*);
-static lean_object* l_myMacro____x40_Init_Core___hyg_1576____closed__1;
 static lean_object* l_myMacro____x40_Init_Core___hyg_175____closed__5;
 static lean_object* l_myMacro____x40_Init_Core___hyg_175____closed__14;
 lean_object* l_prodHasDecidableLt___rarg___boxed(lean_object*, lean_object*, lean_object*, lean_object*, lean_object*, lean_object*);
 lean_object* l_Quot_rec(lean_object*, lean_object*, lean_object*);
 lean_object* l_Decidable_byCases_match__1___rarg___boxed(lean_object*, lean_object*, lean_object*);
 lean_object* l_Subtype_instDecidableEqSubtype_match__1___rarg(lean_object*, lean_object*);
-static lean_object* l_myMacro____x40_Init_Core___hyg_1576____closed__2;
 lean_object* l_Task_Priority_max;
 lean_object* l_instDecidableEqSum_match__1(lean_object*, lean_object*, lean_object*);
 lean_object* l_Decidable_byCases_match__1(lean_object*, lean_object*);
@@ -284,11 +282,13 @@ lean_object* l_Prod_map(lean_object*, lean_object*, lean_object*, lean_object*);
 static lean_object* l_term___x21_x3d_____closed__4;
 lean_object* l_instDecidableEqProd_match__1___rarg___boxed(lean_object*, lean_object*, lean_object*);
 lean_object* l_Quot_indep___rarg(lean_object*, lean_object*);
+static lean_object* l_myMacro____x40_Init_Core___hyg_1981____closed__5;
 lean_object* l_Eq_mp___rarg___boxed(lean_object*);
 static lean_object* l_term___u2248_____closed__3;
 static lean_object* l_myMacro____x40_Init_Core___hyg_1147____closed__9;
 lean_object* l_Decidable_byCases___rarg(uint8_t, lean_object*, lean_object*);
 lean_object* l_prodHasDecidableLt(lean_object*, lean_object*, lean_object*, lean_object*);
+static lean_object* l_myMacro____x40_Init_Core___hyg_1580____closed__2;
 lean_object* l_decidableOfDecidableOfIff___rarg___boxed(lean_object*, lean_object*);
 lean_object* l_Subtype_instInhabitedSubtype___rarg(lean_object*, lean_object*);
 lean_object* l_flip(lean_object*, lean_object*, lean_object*);
@@ -296,18 +296,16 @@ static lean_object* l_term___u2248_____closed__6;
 lean_object* l_Lean_Syntax_getArg(lean_object*, lean_object*);
 lean_object* l_Quotient_recOnSubsingleton_u2082(lean_object*, lean_object*, lean_object*, lean_object*, lean_object*, lean_object*);
 lean_object* l_Decidable_byCases(lean_object*, lean_object*);
+static lean_object* l_myMacro____x40_Init_Core___hyg_1580____closed__1;
 lean_object* l_inline___rarg(lean_object*);
 static lean_object* l_myMacro____x40_Init_Core___hyg_175____closed__1;
 lean_object* l_instDecidableEqSum_match__1___rarg(lean_object*, lean_object*, lean_object*, lean_object*, lean_object*, lean_object*);
-static lean_object* l_myMacro____x40_Init_Core___hyg_1576____closed__6;
 lean_object* l___private_Init_Core_0__funSetoid(lean_object*, lean_object*);
 lean_object* l_Sum_inhabitedRight(lean_object*, lean_object*);
 uint8_t l_strictAnd(uint8_t, uint8_t);
 lean_object* l_Quotient_liftOn_u2082___rarg(lean_object*, lean_object*, lean_object*, lean_object*);
 static lean_object* l_term___u2248_____closed__2;
 uint8_t l_instDecidableArrow___rarg(uint8_t, uint8_t);
-static lean_object* l_myMacro____x40_Init_Core___hyg_1977____closed__5;
-static lean_object* l_myMacro____x40_Init_Core___hyg_1576____closed__4;
 lean_object* l_Squash_mk___rarg(lean_object*);
 static lean_object* l_unexpand____x40_Init_Core___hyg_158____closed__2;
 lean_object* l_instDecidableIte(lean_object*, lean_object*, lean_object*);
@@ -320,6 +318,7 @@ static lean_object* l_myMacro____x40_Init_Core___hyg_175____closed__7;
 lean_object* lean_thunk_get_own(lean_object*);
 lean_object* l_Quotient_hrecOn(lean_object*, lean_object*, lean_object*);
 lean_object* lean_task_pure(lean_object*);
+static lean_object* l_myMacro____x40_Init_Core___hyg_1580____closed__4;
 static lean_object* l_term___u2248_____closed__5;
 lean_object* l___private_Init_Core_0__extfunApp___rarg(lean_object*, lean_object*);
 lean_object* l_Eq_ndrecOn(lean_object*, lean_object*, lean_object*, lean_object*, lean_object*);
@@ -332,6 +331,7 @@ lean_object* l_Thunk_bind(lean_object*, lean_object*);
 lean_object* l_instInhabitedTrue;
 lean_object* l_Quotient_recOn___boxed(lean_object*, lean_object*, lean_object*);
 lean_object* l_Quot_recOn(lean_object*, lean_object*, lean_object*);
+static lean_object* l_myMacro____x40_Init_Core___hyg_1580____closed__6;
 lean_object* l_Quot_hrecOn___rarg(lean_object*, lean_object*, lean_object*);
 lean_object* l_inline___rarg(lean_object* x_1) {
 _start:
@@ -2476,7 +2476,7 @@ x_1 = l_term___x21_x3d_____closed__6;
 return x_1;
 }
 }
-static lean_object* _init_l_myMacro____x40_Init_Core___hyg_1576____closed__1() {
+static lean_object* _init_l_myMacro____x40_Init_Core___hyg_1580____closed__1() {
 _start:
 {
 lean_object* x_1; 
@@ -2484,22 +2484,22 @@ x_1 = lean_mk_string("bne");
 return x_1;
 }
 }
-static lean_object* _init_l_myMacro____x40_Init_Core___hyg_1576____closed__2() {
+static lean_object* _init_l_myMacro____x40_Init_Core___hyg_1580____closed__2() {
 _start:
 {
 lean_object* x_1; lean_object* x_2; 
-x_1 = l_myMacro____x40_Init_Core___hyg_1576____closed__1;
+x_1 = l_myMacro____x40_Init_Core___hyg_1580____closed__1;
 x_2 = lean_string_utf8_byte_size(x_1);
 return x_2;
 }
 }
-static lean_object* _init_l_myMacro____x40_Init_Core___hyg_1576____closed__3() {
+static lean_object* _init_l_myMacro____x40_Init_Core___hyg_1580____closed__3() {
 _start:
 {
 lean_object* x_1; lean_object* x_2; lean_object* x_3; lean_object* x_4; 
-x_1 = l_myMacro____x40_Init_Core___hyg_1576____closed__1;
+x_1 = l_myMacro____x40_Init_Core___hyg_1580____closed__1;
 x_2 = lean_unsigned_to_nat(0u);
-x_3 = l_myMacro____x40_Init_Core___hyg_1576____closed__2;
+x_3 = l_myMacro____x40_Init_Core___hyg_1580____closed__2;
 x_4 = lean_alloc_ctor(0, 3, 0);
 lean_ctor_set(x_4, 0, x_1);
 lean_ctor_set(x_4, 1, x_2);
@@ -2507,41 +2507,41 @@ lean_ctor_set(x_4, 2, x_3);
 return x_4;
 }
 }
-static lean_object* _init_l_myMacro____x40_Init_Core___hyg_1576____closed__4() {
+static lean_object* _init_l_myMacro____x40_Init_Core___hyg_1580____closed__4() {
 _start:
 {
 lean_object* x_1; lean_object* x_2; lean_object* x_3; 
 x_1 = lean_box(0);
-x_2 = l_myMacro____x40_Init_Core___hyg_1576____closed__1;
+x_2 = l_myMacro____x40_Init_Core___hyg_1580____closed__1;
 x_3 = lean_name_mk_string(x_1, x_2);
 return x_3;
 }
 }
-static lean_object* _init_l_myMacro____x40_Init_Core___hyg_1576____closed__5() {
+static lean_object* _init_l_myMacro____x40_Init_Core___hyg_1580____closed__5() {
 _start:
 {
 lean_object* x_1; lean_object* x_2; lean_object* x_3; 
 x_1 = lean_box(0);
-x_2 = l_myMacro____x40_Init_Core___hyg_1576____closed__4;
+x_2 = l_myMacro____x40_Init_Core___hyg_1580____closed__4;
 x_3 = lean_alloc_ctor(0, 2, 0);
 lean_ctor_set(x_3, 0, x_2);
 lean_ctor_set(x_3, 1, x_1);
 return x_3;
 }
 }
-static lean_object* _init_l_myMacro____x40_Init_Core___hyg_1576____closed__6() {
+static lean_object* _init_l_myMacro____x40_Init_Core___hyg_1580____closed__6() {
 _start:
 {
 lean_object* x_1; lean_object* x_2; lean_object* x_3; 
 x_1 = lean_box(0);
-x_2 = l_myMacro____x40_Init_Core___hyg_1576____closed__5;
+x_2 = l_myMacro____x40_Init_Core___hyg_1580____closed__5;
 x_3 = lean_alloc_ctor(1, 2, 0);
 lean_ctor_set(x_3, 0, x_2);
 lean_ctor_set(x_3, 1, x_1);
 return x_3;
 }
 }
-lean_object* l_myMacro____x40_Init_Core___hyg_1576_(lean_object* x_1, lean_object* x_2, lean_object* x_3) {
+lean_object* l_myMacro____x40_Init_Core___hyg_1580_(lean_object* x_1, lean_object* x_2, lean_object* x_3) {
 _start:
 {
 lean_object* x_4; uint8_t x_5; 
@@ -2579,10 +2579,10 @@ lean_inc(x_15);
 x_16 = lean_ctor_get(x_2, 1);
 lean_inc(x_16);
 lean_dec(x_2);
-x_17 = l_myMacro____x40_Init_Core___hyg_1576____closed__4;
+x_17 = l_myMacro____x40_Init_Core___hyg_1580____closed__4;
 x_18 = l_Lean_addMacroScope(x_16, x_17, x_15);
-x_19 = l_myMacro____x40_Init_Core___hyg_1576____closed__3;
-x_20 = l_myMacro____x40_Init_Core___hyg_1576____closed__6;
+x_19 = l_myMacro____x40_Init_Core___hyg_1580____closed__3;
+x_20 = l_myMacro____x40_Init_Core___hyg_1580____closed__6;
 x_21 = lean_alloc_ctor(3, 4, 0);
 lean_ctor_set(x_21, 0, x_14);
 lean_ctor_set(x_21, 1, x_19);
@@ -2617,10 +2617,10 @@ lean_inc(x_33);
 x_34 = lean_ctor_get(x_2, 1);
 lean_inc(x_34);
 lean_dec(x_2);
-x_35 = l_myMacro____x40_Init_Core___hyg_1576____closed__4;
+x_35 = l_myMacro____x40_Init_Core___hyg_1580____closed__4;
 x_36 = l_Lean_addMacroScope(x_34, x_35, x_33);
-x_37 = l_myMacro____x40_Init_Core___hyg_1576____closed__3;
-x_38 = l_myMacro____x40_Init_Core___hyg_1576____closed__6;
+x_37 = l_myMacro____x40_Init_Core___hyg_1580____closed__3;
+x_38 = l_myMacro____x40_Init_Core___hyg_1580____closed__6;
 x_39 = lean_alloc_ctor(3, 4, 0);
 lean_ctor_set(x_39, 0, x_31);
 lean_ctor_set(x_39, 1, x_37);
@@ -2647,7 +2647,7 @@ return x_49;
 }
 }
 }
-lean_object* l_unexpand____x40_Init_Core___hyg_1559_(lean_object* x_1, lean_object* x_2) {
+lean_object* l_unexpand____x40_Init_Core___hyg_1563_(lean_object* x_1, lean_object* x_2) {
 _start:
 {
 lean_object* x_3; uint8_t x_4; 
@@ -2880,7 +2880,7 @@ x_1 = l_term___u2260_____closed__6;
 return x_1;
 }
 }
-static lean_object* _init_l_myMacro____x40_Init_Core___hyg_1977____closed__1() {
+static lean_object* _init_l_myMacro____x40_Init_Core___hyg_1981____closed__1() {
 _start:
 {
 lean_object* x_1; 
@@ -2888,22 +2888,22 @@ x_1 = lean_mk_string("Ne");
 return x_1;
 }
 }
-static lean_object* _init_l_myMacro____x40_Init_Core___hyg_1977____closed__2() {
+static lean_object* _init_l_myMacro____x40_Init_Core___hyg_1981____closed__2() {
 _start:
 {
 lean_object* x_1; lean_object* x_2; 
-x_1 = l_myMacro____x40_Init_Core___hyg_1977____closed__1;
+x_1 = l_myMacro____x40_Init_Core___hyg_1981____closed__1;
 x_2 = lean_string_utf8_byte_size(x_1);
 return x_2;
 }
 }
-static lean_object* _init_l_myMacro____x40_Init_Core___hyg_1977____closed__3() {
+static lean_object* _init_l_myMacro____x40_Init_Core___hyg_1981____closed__3() {
 _start:
 {
 lean_object* x_1; lean_object* x_2; lean_object* x_3; lean_object* x_4; 
-x_1 = l_myMacro____x40_Init_Core___hyg_1977____closed__1;
+x_1 = l_myMacro____x40_Init_Core___hyg_1981____closed__1;
 x_2 = lean_unsigned_to_nat(0u);
-x_3 = l_myMacro____x40_Init_Core___hyg_1977____closed__2;
+x_3 = l_myMacro____x40_Init_Core___hyg_1981____closed__2;
 x_4 = lean_alloc_ctor(0, 3, 0);
 lean_ctor_set(x_4, 0, x_1);
 lean_ctor_set(x_4, 1, x_2);
@@ -2911,41 +2911,41 @@ lean_ctor_set(x_4, 2, x_3);
 return x_4;
 }
 }
-static lean_object* _init_l_myMacro____x40_Init_Core___hyg_1977____closed__4() {
+static lean_object* _init_l_myMacro____x40_Init_Core___hyg_1981____closed__4() {
 _start:
 {
 lean_object* x_1; lean_object* x_2; lean_object* x_3; 
 x_1 = lean_box(0);
-x_2 = l_myMacro____x40_Init_Core___hyg_1977____closed__1;
+x_2 = l_myMacro____x40_Init_Core___hyg_1981____closed__1;
 x_3 = lean_name_mk_string(x_1, x_2);
 return x_3;
 }
 }
-static lean_object* _init_l_myMacro____x40_Init_Core___hyg_1977____closed__5() {
+static lean_object* _init_l_myMacro____x40_Init_Core___hyg_1981____closed__5() {
 _start:
 {
 lean_object* x_1; lean_object* x_2; lean_object* x_3; 
 x_1 = lean_box(0);
-x_2 = l_myMacro____x40_Init_Core___hyg_1977____closed__4;
+x_2 = l_myMacro____x40_Init_Core___hyg_1981____closed__4;
 x_3 = lean_alloc_ctor(0, 2, 0);
 lean_ctor_set(x_3, 0, x_2);
 lean_ctor_set(x_3, 1, x_1);
 return x_3;
 }
 }
-static lean_object* _init_l_myMacro____x40_Init_Core___hyg_1977____closed__6() {
+static lean_object* _init_l_myMacro____x40_Init_Core___hyg_1981____closed__6() {
 _start:
 {
 lean_object* x_1; lean_object* x_2; lean_object* x_3; 
 x_1 = lean_box(0);
-x_2 = l_myMacro____x40_Init_Core___hyg_1977____closed__5;
+x_2 = l_myMacro____x40_Init_Core___hyg_1981____closed__5;
 x_3 = lean_alloc_ctor(1, 2, 0);
 lean_ctor_set(x_3, 0, x_2);
 lean_ctor_set(x_3, 1, x_1);
 return x_3;
 }
 }
-lean_object* l_myMacro____x40_Init_Core___hyg_1977_(lean_object* x_1, lean_object* x_2, lean_object* x_3) {
+lean_object* l_myMacro____x40_Init_Core___hyg_1981_(lean_object* x_1, lean_object* x_2, lean_object* x_3) {
 _start:
 {
 lean_object* x_4; uint8_t x_5; 
@@ -2983,10 +2983,10 @@ lean_inc(x_15);
 x_16 = lean_ctor_get(x_2, 1);
 lean_inc(x_16);
 lean_dec(x_2);
-x_17 = l_myMacro____x40_Init_Core___hyg_1977____closed__4;
+x_17 = l_myMacro____x40_Init_Core___hyg_1981____closed__4;
 x_18 = l_Lean_addMacroScope(x_16, x_17, x_15);
-x_19 = l_myMacro____x40_Init_Core___hyg_1977____closed__3;
-x_20 = l_myMacro____x40_Init_Core___hyg_1977____closed__6;
+x_19 = l_myMacro____x40_Init_Core___hyg_1981____closed__3;
+x_20 = l_myMacro____x40_Init_Core___hyg_1981____closed__6;
 x_21 = lean_alloc_ctor(3, 4, 0);
 lean_ctor_set(x_21, 0, x_14);
 lean_ctor_set(x_21, 1, x_19);
@@ -3021,10 +3021,10 @@ lean_inc(x_33);
 x_34 = lean_ctor_get(x_2, 1);
 lean_inc(x_34);
 lean_dec(x_2);
-x_35 = l_myMacro____x40_Init_Core___hyg_1977____closed__4;
+x_35 = l_myMacro____x40_Init_Core___hyg_1981____closed__4;
 x_36 = l_Lean_addMacroScope(x_34, x_35, x_33);
-x_37 = l_myMacro____x40_Init_Core___hyg_1977____closed__3;
-x_38 = l_myMacro____x40_Init_Core___hyg_1977____closed__6;
+x_37 = l_myMacro____x40_Init_Core___hyg_1981____closed__3;
+x_38 = l_myMacro____x40_Init_Core___hyg_1981____closed__6;
 x_39 = lean_alloc_ctor(3, 4, 0);
 lean_ctor_set(x_39, 0, x_31);
 lean_ctor_set(x_39, 1, x_37);
@@ -3051,7 +3051,7 @@ return x_49;
 }
 }
 }
-lean_object* l_unexpand____x40_Init_Core___hyg_1960_(lean_object* x_1, lean_object* x_2) {
+lean_object* l_unexpand____x40_Init_Core___hyg_1964_(lean_object* x_1, lean_object* x_2) {
 _start:
 {
 lean_object* x_3; uint8_t x_4; 
@@ -4841,18 +4841,18 @@ l_term___x21_x3d_____closed__6 = _init_l_term___x21_x3d_____closed__6();
 lean_mark_persistent(l_term___x21_x3d_____closed__6);
 l_term___x21_x3d__ = _init_l_term___x21_x3d__();
 lean_mark_persistent(l_term___x21_x3d__);
-l_myMacro____x40_Init_Core___hyg_1576____closed__1 = _init_l_myMacro____x40_Init_Core___hyg_1576____closed__1();
-lean_mark_persistent(l_myMacro____x40_Init_Core___hyg_1576____closed__1);
-l_myMacro____x40_Init_Core___hyg_1576____closed__2 = _init_l_myMacro____x40_Init_Core___hyg_1576____closed__2();
-lean_mark_persistent(l_myMacro____x40_Init_Core___hyg_1576____closed__2);
-l_myMacro____x40_Init_Core___hyg_1576____closed__3 = _init_l_myMacro____x40_Init_Core___hyg_1576____closed__3();
-lean_mark_persistent(l_myMacro____x40_Init_Core___hyg_1576____closed__3);
-l_myMacro____x40_Init_Core___hyg_1576____closed__4 = _init_l_myMacro____x40_Init_Core___hyg_1576____closed__4();
-lean_mark_persistent(l_myMacro____x40_Init_Core___hyg_1576____closed__4);
-l_myMacro____x40_Init_Core___hyg_1576____closed__5 = _init_l_myMacro____x40_Init_Core___hyg_1576____closed__5();
-lean_mark_persistent(l_myMacro____x40_Init_Core___hyg_1576____closed__5);
-l_myMacro____x40_Init_Core___hyg_1576____closed__6 = _init_l_myMacro____x40_Init_Core___hyg_1576____closed__6();
-lean_mark_persistent(l_myMacro____x40_Init_Core___hyg_1576____closed__6);
+l_myMacro____x40_Init_Core___hyg_1580____closed__1 = _init_l_myMacro____x40_Init_Core___hyg_1580____closed__1();
+lean_mark_persistent(l_myMacro____x40_Init_Core___hyg_1580____closed__1);
+l_myMacro____x40_Init_Core___hyg_1580____closed__2 = _init_l_myMacro____x40_Init_Core___hyg_1580____closed__2();
+lean_mark_persistent(l_myMacro____x40_Init_Core___hyg_1580____closed__2);
+l_myMacro____x40_Init_Core___hyg_1580____closed__3 = _init_l_myMacro____x40_Init_Core___hyg_1580____closed__3();
+lean_mark_persistent(l_myMacro____x40_Init_Core___hyg_1580____closed__3);
+l_myMacro____x40_Init_Core___hyg_1580____closed__4 = _init_l_myMacro____x40_Init_Core___hyg_1580____closed__4();
+lean_mark_persistent(l_myMacro____x40_Init_Core___hyg_1580____closed__4);
+l_myMacro____x40_Init_Core___hyg_1580____closed__5 = _init_l_myMacro____x40_Init_Core___hyg_1580____closed__5();
+lean_mark_persistent(l_myMacro____x40_Init_Core___hyg_1580____closed__5);
+l_myMacro____x40_Init_Core___hyg_1580____closed__6 = _init_l_myMacro____x40_Init_Core___hyg_1580____closed__6();
+lean_mark_persistent(l_myMacro____x40_Init_Core___hyg_1580____closed__6);
 l_term___u2260_____closed__1 = _init_l_term___u2260_____closed__1();
 lean_mark_persistent(l_term___u2260_____closed__1);
 l_term___u2260_____closed__2 = _init_l_term___u2260_____closed__2();
@@ -4867,18 +4867,18 @@ l_term___u2260_____closed__6 = _init_l_term___u2260_____closed__6();
 lean_mark_persistent(l_term___u2260_____closed__6);
 l_term___u2260__ = _init_l_term___u2260__();
 lean_mark_persistent(l_term___u2260__);
-l_myMacro____x40_Init_Core___hyg_1977____closed__1 = _init_l_myMacro____x40_Init_Core___hyg_1977____closed__1();
-lean_mark_persistent(l_myMacro____x40_Init_Core___hyg_1977____closed__1);
-l_myMacro____x40_Init_Core___hyg_1977____closed__2 = _init_l_myMacro____x40_Init_Core___hyg_1977____closed__2();
-lean_mark_persistent(l_myMacro____x40_Init_Core___hyg_1977____closed__2);
-l_myMacro____x40_Init_Core___hyg_1977____closed__3 = _init_l_myMacro____x40_Init_Core___hyg_1977____closed__3();
-lean_mark_persistent(l_myMacro____x40_Init_Core___hyg_1977____closed__3);
-l_myMacro____x40_Init_Core___hyg_1977____closed__4 = _init_l_myMacro____x40_Init_Core___hyg_1977____closed__4();
-lean_mark_persistent(l_myMacro____x40_Init_Core___hyg_1977____closed__4);
-l_myMacro____x40_Init_Core___hyg_1977____closed__5 = _init_l_myMacro____x40_Init_Core___hyg_1977____closed__5();
-lean_mark_persistent(l_myMacro____x40_Init_Core___hyg_1977____closed__5);
-l_myMacro____x40_Init_Core___hyg_1977____closed__6 = _init_l_myMacro____x40_Init_Core___hyg_1977____closed__6();
-lean_mark_persistent(l_myMacro____x40_Init_Core___hyg_1977____closed__6);
+l_myMacro____x40_Init_Core___hyg_1981____closed__1 = _init_l_myMacro____x40_Init_Core___hyg_1981____closed__1();
+lean_mark_persistent(l_myMacro____x40_Init_Core___hyg_1981____closed__1);
+l_myMacro____x40_Init_Core___hyg_1981____closed__2 = _init_l_myMacro____x40_Init_Core___hyg_1981____closed__2();
+lean_mark_persistent(l_myMacro____x40_Init_Core___hyg_1981____closed__2);
+l_myMacro____x40_Init_Core___hyg_1981____closed__3 = _init_l_myMacro____x40_Init_Core___hyg_1981____closed__3();
+lean_mark_persistent(l_myMacro____x40_Init_Core___hyg_1981____closed__3);
+l_myMacro____x40_Init_Core___hyg_1981____closed__4 = _init_l_myMacro____x40_Init_Core___hyg_1981____closed__4();
+lean_mark_persistent(l_myMacro____x40_Init_Core___hyg_1981____closed__4);
+l_myMacro____x40_Init_Core___hyg_1981____closed__5 = _init_l_myMacro____x40_Init_Core___hyg_1981____closed__5();
+lean_mark_persistent(l_myMacro____x40_Init_Core___hyg_1981____closed__5);
+l_myMacro____x40_Init_Core___hyg_1981____closed__6 = _init_l_myMacro____x40_Init_Core___hyg_1981____closed__6();
+lean_mark_persistent(l_myMacro____x40_Init_Core___hyg_1981____closed__6);
 l_instDecidableTrue = _init_l_instDecidableTrue();
 l_instDecidableFalse = _init_l_instDecidableFalse();
 l_instInhabitedProp = _init_l_instInhabitedProp();
