stage0/stdlib/Lean/Compiler/ConstFolding.c
@@ -14,7 +14,6 @@
 extern "C" {
 #endif
 static lean_object* l_Lean_Compiler_unFoldFns___closed__5;
-static lean_object* l_Lean_Compiler_mkNatLt___closed__12;
 static lean_object* l_Lean_Compiler_unFoldFns___closed__3;
 static lean_object* l_Lean_Compiler_preUIntBinFoldFns___closed__5;
 lean_object* l_Lean_Compiler_mkNatLe(lean_object*, lean_object*);
@@ -105,7 +104,6 @@ lean_object* l_Lean_Compiler_foldNatDecLe___boxed(lean_object*, lean_object*, le
 lean_object* l_Lean_Compiler_foldNatDiv(uint8_t);
 extern lean_object* l_Lean_levelZero;
 lean_object* lean_nat_add(lean_object*, lean_object*);
-static lean_object* l_Lean_Compiler_mkNatLe___closed__9;
 static lean_object* l_Lean_Compiler_preUIntBinFoldFns___closed__19;
 lean_object* l_Lean_Compiler_mkUInt32Lit(lean_object*);
 static lean_object* l_Lean_Compiler_numScalarTypes___closed__17;
@@ -2493,32 +2491,24 @@ return x_3;
 static lean_object* _init_l_Lean_Compiler_mkNatLt___closed__7() {
 _start:
 {
-lean_object* x_1; 
-x_1 = lean_mk_string("less");
-return x_1;
+lean_object* x_1; lean_object* x_2; lean_object* x_3; 
+x_1 = l_Lean_Compiler_mkNatEq___closed__6;
+x_2 = l_Lean_Compiler_mkNatLt___closed__3;
+x_3 = lean_name_mk_string(x_1, x_2);
+return x_3;
 }
 }
 static lean_object* _init_l_Lean_Compiler_mkNatLt___closed__8() {
 _start:
 {
 lean_object* x_1; lean_object* x_2; lean_object* x_3; 
-x_1 = l_Lean_Compiler_mkNatEq___closed__6;
-x_2 = l_Lean_Compiler_mkNatLt___closed__7;
-x_3 = lean_name_mk_string(x_1, x_2);
-return x_3;
-}
-}
-static lean_object* _init_l_Lean_Compiler_mkNatLt___closed__9() {
-_start:
-{
-lean_object* x_1; lean_object* x_2; lean_object* x_3; 
 x_1 = lean_box(0);
-x_2 = l_Lean_Compiler_mkNatLt___closed__8;
+x_2 = l_Lean_Compiler_mkNatLt___closed__7;
 x_3 = l_Lean_mkConst(x_2, x_1);
 return x_3;
 }
 }
-static lean_object* _init_l_Lean_Compiler_mkNatLt___closed__10() {
+static lean_object* _init_l_Lean_Compiler_mkNatLt___closed__9() {
 _start:
 {
 lean_object* x_1; lean_object* x_2; 
@@ -2527,22 +2517,22 @@ x_2 = lean_mk_empty_array_with_capacity(x_1);
 return x_2;
 }
 }
-static lean_object* _init_l_Lean_Compiler_mkNatLt___closed__11() {
+static lean_object* _init_l_Lean_Compiler_mkNatLt___closed__10() {
 _start:
 {
 lean_object* x_1; lean_object* x_2; lean_object* x_3; 
-x_1 = l_Lean_Compiler_mkNatLt___closed__10;
+x_1 = l_Lean_Compiler_mkNatLt___closed__9;
 x_2 = l_Lean_Compiler_mkNatEq___closed__7;
 x_3 = lean_array_push(x_1, x_2);
 return x_3;
 }
 }
-static lean_object* _init_l_Lean_Compiler_mkNatLt___closed__12() {
+static lean_object* _init_l_Lean_Compiler_mkNatLt___closed__11() {
 _start:
 {
 lean_object* x_1; lean_object* x_2; lean_object* x_3; 
-x_1 = l_Lean_Compiler_mkNatLt___closed__11;
-x_2 = l_Lean_Compiler_mkNatLt___closed__9;
+x_1 = l_Lean_Compiler_mkNatLt___closed__10;
+x_2 = l_Lean_Compiler_mkNatLt___closed__8;
 x_3 = lean_array_push(x_1, x_2);
 return x_3;
 }
@@ -2551,7 +2541,7 @@ lean_object* l_Lean_Compiler_mkNatLt(lean_object* x_1, lean_object* x_2) {
 _start:
 {
 lean_object* x_3; lean_object* x_4; lean_object* x_5; lean_object* x_6; lean_object* x_7; 
-x_3 = l_Lean_Compiler_mkNatLt___closed__12;
+x_3 = l_Lean_Compiler_mkNatLt___closed__11;
 x_4 = lean_array_push(x_3, x_1);
 x_5 = lean_array_push(x_4, x_2);
 x_6 = l_Lean_Compiler_mkNatLt___closed__6;
@@ -2608,18 +2598,20 @@ return x_3;
 static lean_object* _init_l_Lean_Compiler_mkNatLe___closed__6() {
 _start:
 {
-lean_object* x_1; 
-x_1 = lean_mk_string("lessEq");
-return x_1;
+lean_object* x_1; lean_object* x_2; lean_object* x_3; 
+x_1 = l_Lean_Compiler_mkNatEq___closed__6;
+x_2 = l_Lean_Compiler_mkNatLe___closed__3;
+x_3 = lean_name_mk_string(x_1, x_2);
+return x_3;
 }
 }
 static lean_object* _init_l_Lean_Compiler_mkNatLe___closed__7() {
 _start:
 {
 lean_object* x_1; lean_object* x_2; lean_object* x_3; 
-x_1 = l_Lean_Compiler_mkNatEq___closed__6;
+x_1 = lean_box(0);
 x_2 = l_Lean_Compiler_mkNatLe___closed__6;
-x_3 = lean_name_mk_string(x_1, x_2);
+x_3 = l_Lean_mkConst(x_2, x_1);
 return x_3;
 }
 }
@@ -2627,18 +2619,8 @@ static lean_object* _init_l_Lean_Compiler_mkNatLe___closed__8() {
 _start:
 {
 lean_object* x_1; lean_object* x_2; lean_object* x_3; 
-x_1 = lean_box(0);
+x_1 = l_Lean_Compiler_mkNatLt___closed__10;
 x_2 = l_Lean_Compiler_mkNatLe___closed__7;
-x_3 = l_Lean_mkConst(x_2, x_1);
-return x_3;
-}
-}
-static lean_object* _init_l_Lean_Compiler_mkNatLe___closed__9() {
-_start:
-{
-lean_object* x_1; lean_object* x_2; lean_object* x_3; 
-x_1 = l_Lean_Compiler_mkNatLt___closed__11;
-x_2 = l_Lean_Compiler_mkNatLe___closed__8;
 x_3 = lean_array_push(x_1, x_2);
 return x_3;
 }
@@ -2647,7 +2629,7 @@ lean_object* l_Lean_Compiler_mkNatLe(lean_object* x_1, lean_object* x_2) {
 _start:
 {
 lean_object* x_3; lean_object* x_4; lean_object* x_5; lean_object* x_6; lean_object* x_7; 
-x_3 = l_Lean_Compiler_mkNatLe___closed__9;
+x_3 = l_Lean_Compiler_mkNatLe___closed__8;
 x_4 = lean_array_push(x_3, x_1);
 x_5 = lean_array_push(x_4, x_2);
 x_6 = l_Lean_Compiler_mkNatLe___closed__5;
@@ -5345,8 +5327,6 @@ l_Lean_Compiler_mkNatLt___closed__10 = _init_l_Lean_Compiler_mkNatLt___closed__1
 lean_mark_persistent(l_Lean_Compiler_mkNatLt___closed__10);
 l_Lean_Compiler_mkNatLt___closed__11 = _init_l_Lean_Compiler_mkNatLt___closed__11();
 lean_mark_persistent(l_Lean_Compiler_mkNatLt___closed__11);
-l_Lean_Compiler_mkNatLt___closed__12 = _init_l_Lean_Compiler_mkNatLt___closed__12();
-lean_mark_persistent(l_Lean_Compiler_mkNatLt___closed__12);
 l_Lean_Compiler_mkNatLe___closed__1 = _init_l_Lean_Compiler_mkNatLe___closed__1();
 lean_mark_persistent(l_Lean_Compiler_mkNatLe___closed__1);
 l_Lean_Compiler_mkNatLe___closed__2 = _init_l_Lean_Compiler_mkNatLe___closed__2();
@@ -5363,8 +5343,6 @@ l_Lean_Compiler_mkNatLe___closed__7 = _init_l_Lean_Compiler_mkNatLe___closed__7(
 lean_mark_persistent(l_Lean_Compiler_mkNatLe___closed__7);
 l_Lean_Compiler_mkNatLe___closed__8 = _init_l_Lean_Compiler_mkNatLe___closed__8();
 lean_mark_persistent(l_Lean_Compiler_mkNatLe___closed__8);
-l_Lean_Compiler_mkNatLe___closed__9 = _init_l_Lean_Compiler_mkNatLe___closed__9();
-lean_mark_persistent(l_Lean_Compiler_mkNatLe___closed__9);
 l_Lean_Compiler_toDecidableExpr___closed__1 = _init_l_Lean_Compiler_toDecidableExpr___closed__1();
 lean_mark_persistent(l_Lean_Compiler_toDecidableExpr___closed__1);
 l_Lean_Compiler_toDecidableExpr___closed__2 = _init_l_Lean_Compiler_toDecidableExpr___closed__2();
