stage0/stdlib/Lean/Elab/Declaration.c
@@ -400,7 +400,6 @@ lean_object* l___private_Lean_Elab_Declaration_0__Lean_Elab_Command_inductiveSyn
 uint8_t l_Lean_Elab_Modifiers_isPrivate(lean_object*);
 static lean_object* l_Lean_Elab_Command_expandInitCmd___closed__9;
 lean_object* l_Lean_Elab_Term_addAutoBoundImplicits(lean_object*, lean_object*, lean_object*, lean_object*, lean_object*, lean_object*, lean_object*, lean_object*);
-static lean_object* l___private_Lean_Elab_Declaration_0__Lean_Elab_Command_isMutualPreambleCommand___closed__11;
 static lean_object* l_Lean_Elab_Command_expandInitCmd___closed__8;
 lean_object* l_Lean_Syntax_getArg(lean_object*, lean_object*);
 static lean_object* l_Lean_Elab_Command_expandInitCmd___lambda__1___closed__52;
@@ -458,7 +457,6 @@ lean_object* l_Array_mapMUnsafe_map___at___private_Lean_Elab_Declaration_0__Lean
 lean_object* l_Lean_Elab_Command_elabAxiom_match__1(lean_object*);
 static lean_object* l_Lean_Elab_Command_expandInitCmd___closed__1;
 lean_object* l_Lean_Syntax_formatStxAux(lean_object*, uint8_t, lean_object*, lean_object*);
-static lean_object* l___private_Lean_Elab_Declaration_0__Lean_Elab_Command_isMutualPreambleCommand___closed__12;
 lean_object* l_Lean_Elab_Command_expandInitCmd___boxed(lean_object*, lean_object*, lean_object*, lean_object*);
 static lean_object* l_Lean_Elab_Command_expandInitCmd___lambda__1___closed__37;
 static lean_object* l_Array_mapMUnsafe_map___at___private_Lean_Elab_Declaration_0__Lean_Elab_Command_inductiveSyntaxToView___spec__3___lambda__2___closed__2;
@@ -5375,7 +5373,7 @@ static lean_object* _init_l___private_Lean_Elab_Declaration_0__Lean_Elab_Command
 _start:
 {
 lean_object* x_1; 
-x_1 = lean_mk_string("variables");
+x_1 = lean_mk_string("universe");
 return x_1;
 }
 }
@@ -5393,7 +5391,7 @@ static lean_object* _init_l___private_Lean_Elab_Declaration_0__Lean_Elab_Command
 _start:
 {
 lean_object* x_1; 
-x_1 = lean_mk_string("universe");
+x_1 = lean_mk_string("check");
 return x_1;
 }
 }
@@ -5411,7 +5409,7 @@ static lean_object* _init_l___private_Lean_Elab_Declaration_0__Lean_Elab_Command
 _start:
 {
 lean_object* x_1; 
-x_1 = lean_mk_string("check");
+x_1 = lean_mk_string("set_option");
 return x_1;
 }
 }
@@ -5429,7 +5427,7 @@ static lean_object* _init_l___private_Lean_Elab_Declaration_0__Lean_Elab_Command
 _start:
 {
 lean_object* x_1; 
-x_1 = lean_mk_string("set_option");
+x_1 = lean_mk_string("open");
 return x_1;
 }
 }
@@ -5439,24 +5437,6 @@ _start:
 lean_object* x_1; lean_object* x_2; lean_object* x_3; 
 x_1 = l_Lean_Elab_Command_expandDeclNamespace_x3f___closed__6;
 x_2 = l___private_Lean_Elab_Declaration_0__Lean_Elab_Command_isMutualPreambleCommand___closed__9;
-x_3 = lean_name_mk_string(x_1, x_2);
-return x_3;
-}
-}
-static lean_object* _init_l___private_Lean_Elab_Declaration_0__Lean_Elab_Command_isMutualPreambleCommand___closed__11() {
-_start:
-{
-lean_object* x_1; 
-x_1 = lean_mk_string("open");
-return x_1;
-}
-}
-static lean_object* _init_l___private_Lean_Elab_Declaration_0__Lean_Elab_Command_isMutualPreambleCommand___closed__12() {
-_start:
-{
-lean_object* x_1; lean_object* x_2; lean_object* x_3; 
-x_1 = l_Lean_Elab_Command_expandDeclNamespace_x3f___closed__6;
-x_2 = l___private_Lean_Elab_Declaration_0__Lean_Elab_Command_isMutualPreambleCommand___closed__11;
 x_3 = lean_name_mk_string(x_1, x_2);
 return x_3;
 }
@@ -5488,13 +5468,24 @@ if (x_10 == 0)
 lean_object* x_11; uint8_t x_12; 
 x_11 = l___private_Lean_Elab_Declaration_0__Lean_Elab_Command_isMutualPreambleCommand___closed__10;
 x_12 = lean_name_eq(x_2, x_11);
-if (x_12 == 0)
-{
-lean_object* x_13; uint8_t x_14; 
-x_13 = l___private_Lean_Elab_Declaration_0__Lean_Elab_Command_isMutualPreambleCommand___closed__12;
-x_14 = lean_name_eq(x_2, x_13);
 lean_dec(x_2);
+return x_12;
+}
+else
+{
+uint8_t x_13; 
+lean_dec(x_2);
+x_13 = 1;
+return x_13;
+}
+}
+else
+{
+uint8_t x_14; 
+lean_dec(x_2);
+x_14 = 1;
 return x_14;
+}
 }
 else
 {
@@ -5510,30 +5501,6 @@ uint8_t x_16;
 lean_dec(x_2);
 x_16 = 1;
 return x_16;
-}
-}
-else
-{
-uint8_t x_17; 
-lean_dec(x_2);
-x_17 = 1;
-return x_17;
-}
-}
-else
-{
-uint8_t x_18; 
-lean_dec(x_2);
-x_18 = 1;
-return x_18;
-}
-}
-else
-{
-uint8_t x_19; 
-lean_dec(x_2);
-x_19 = 1;
-return x_19;
 }
 }
 }
@@ -11651,10 +11618,6 @@ l___private_Lean_Elab_Declaration_0__Lean_Elab_Command_isMutualPreambleCommand__
 lean_mark_persistent(l___private_Lean_Elab_Declaration_0__Lean_Elab_Command_isMutualPreambleCommand___closed__9);
 l___private_Lean_Elab_Declaration_0__Lean_Elab_Command_isMutualPreambleCommand___closed__10 = _init_l___private_Lean_Elab_Declaration_0__Lean_Elab_Command_isMutualPreambleCommand___closed__10();
 lean_mark_persistent(l___private_Lean_Elab_Declaration_0__Lean_Elab_Command_isMutualPreambleCommand___closed__10);
-l___private_Lean_Elab_Declaration_0__Lean_Elab_Command_isMutualPreambleCommand___closed__11 = _init_l___private_Lean_Elab_Declaration_0__Lean_Elab_Command_isMutualPreambleCommand___closed__11();
-lean_mark_persistent(l___private_Lean_Elab_Declaration_0__Lean_Elab_Command_isMutualPreambleCommand___closed__11);
-l___private_Lean_Elab_Declaration_0__Lean_Elab_Command_isMutualPreambleCommand___closed__12 = _init_l___private_Lean_Elab_Declaration_0__Lean_Elab_Command_isMutualPreambleCommand___closed__12();
-lean_mark_persistent(l___private_Lean_Elab_Declaration_0__Lean_Elab_Command_isMutualPreambleCommand___closed__12);
 l_Array_forInUnsafe_loop___at_Lean_Elab_Command_expandMutualNamespace___spec__1___closed__1 = _init_l_Array_forInUnsafe_loop___at_Lean_Elab_Command_expandMutualNamespace___spec__1___closed__1();
 lean_mark_persistent(l_Array_forInUnsafe_loop___at_Lean_Elab_Command_expandMutualNamespace___spec__1___closed__1);
 l_Array_forInUnsafe_loop___at_Lean_Elab_Command_expandMutualNamespace___spec__1___closed__2 = _init_l_Array_forInUnsafe_loop___at_Lean_Elab_Command_expandMutualNamespace___spec__1___closed__2();
