stage0/src/Init/Data/Array/InsertionSort.lean
@@ -21,7 +21,7 @@ where
     match he:j with
     | 0    => a
     | j'+1 =>
-      have h' : j' < a.size := by subst j; exact Nat.ltTrans (Nat.ltSuccSelf _) h
+      have h' : j' < a.size := by subst j; exact Nat.lt_trans (Nat.lt_succ_self _) h
       if lt (a.get ⟨j, h⟩) (a.get ⟨j', h'⟩) then
         swapLoop (a.swap ⟨j, h⟩ ⟨j', h'⟩) j' (by rw [size_swap]; assumption done)
       else
