stage0/src/Init/Data/Nat/Div.lean
@@ -9,7 +9,7 @@ import Init.Data.Nat.Basic
 namespace Nat
 
 private def div_rec_lemma {x y : Nat} : 0 < y ∧ y ≤ x → x - y < x :=
-  fun ⟨ypos, ylex⟩ => subLt (Nat.ltOfLtOfLe ypos ylex) ypos
+  fun ⟨ypos, ylex⟩ => sub_lt (Nat.lt_of_lt_of_le ypos ylex) ypos
 
 private def div.F (x : Nat) (f : ∀ x₁, x₁ < x → Nat → Nat) (y : Nat) : Nat :=
   if h : 0 < y ∧ y ≤ x then f (x - y) (div_rec_lemma h) y + 1 else zero
@@ -21,10 +21,10 @@ protected def div (a b : @& Nat) : Nat :=
 instance : Div Nat := ⟨Nat.div⟩
 
 private theorem div_eq_aux (x y : Nat) : x / y = if h : 0 < y ∧ y ≤ x then (x - y) / y + 1 else 0 :=
-  congrFun (WellFounded.fixEq ltWf div.F x) y
+  congrFun (WellFounded.fix_eq ltWf div.F x) y
 
 theorem div_eq (x y : Nat) : x / y = if 0 < y ∧ y ≤ x then (x - y) / y + 1 else 0 :=
-  difEqIf (0 < y ∧ y ≤ x) ((x - y) / y + 1) 0 ▸ div_eq_aux x y
+  dif_eq_if (0 < y ∧ y ≤ x) ((x - y) / y + 1) 0 ▸ div_eq_aux x y
 
 private theorem div.induction.F.{u}
         (C : Nat → Nat → Sort u)
@@ -51,10 +51,10 @@ protected def mod (a b : @& Nat) : Nat :=
 instance : Mod Nat := ⟨Nat.mod⟩
 
 private theorem mod_eq_aux (x y : Nat) : x % y = if h : 0 < y ∧ y ≤ x then (x - y) % y else x :=
-  congrFun (WellFounded.fixEq ltWf mod.F x) y
+  congrFun (WellFounded.fix_eq ltWf mod.F x) y
 
 theorem mod_eq (x y : Nat) : x % y = if 0 < y ∧ y ≤ x then (x - y) % y else x :=
-  difEqIf (0 < y ∧ y ≤ x) ((x - y) % y) x ▸ mod_eq_aux x y
+  dif_eq_if (0 < y ∧ y ≤ x) ((x - y) % y) x ▸ mod_eq_aux x y
 
 theorem mod.inductionOn.{u}
       {motive : Nat → Nat → Sort u}
@@ -66,30 +66,30 @@ theorem mod.inductionOn.{u}
 
 theorem mod_zero (a : Nat) : a % 0 = a :=
   have : (if 0 < 0 ∧ 0 ≤ a then (a - 0) % 0 else a) = a :=
-    have h : ¬ (0 < 0 ∧ 0 ≤ a) := fun ⟨h₁, _⟩ => absurd h₁ (Nat.ltIrrefl _)
-    ifNeg h
+    have h : ¬ (0 < 0 ∧ 0 ≤ a) := fun ⟨h₁, _⟩ => absurd h₁ (Nat.lt_irrefl _)
+    if_neg h
   (mod_eq a 0).symm ▸ this
 
 theorem mod_eq_of_lt {a b : Nat} (h : a < b) : a % b = a :=
   have : (if 0 < b ∧ b ≤ a then (a - b) % b else a) = a :=
-    have h' : ¬(0 < b ∧ b ≤ a) := fun ⟨_, h₁⟩ => absurd h₁ (Nat.notLeOfGt h)
-    ifNeg h'
+    have h' : ¬(0 < b ∧ b ≤ a) := fun ⟨_, h₁⟩ => absurd h₁ (Nat.not_le_of_gt h)
+    if_neg h'
   (mod_eq a b).symm ▸ this
 
 theorem mod_eq_sub_mod {a b : Nat} (h : a ≥ b) : a % b = (a - b) % b :=
-  match eqZeroOrPos b with
+  match eq_zero_or_pos b with
   | Or.inl h₁ => h₁.symm ▸ (Nat.sub_zero a).symm ▸ rfl
-  | Or.inr h₁ => (mod_eq a b).symm ▸ ifPos ⟨h₁, h⟩
+  | Or.inr h₁ => (mod_eq a b).symm ▸ if_pos ⟨h₁, h⟩
 
 theorem mod_lt (x : Nat) {y : Nat} : y > 0 → x % y < y := by
   induction x, y using mod.inductionOn with
   | base x y h₁ =>
     intro h₂
-    have h₁ : ¬ 0 < y ∨ ¬ y ≤ x := Iff.mp (Decidable.notAndIffOrNot _ _) h₁
+    have h₁ : ¬ 0 < y ∨ ¬ y ≤ x := Iff.mp (Decidable.not_and_iff_or_not _ _) h₁
     match h₁ with
     | Or.inl h₁ => exact absurd h₂ h₁
     | Or.inr h₁ =>
-      have hgt : y > x := gtOfNotLe h₁
+      have hgt : y > x := gt_of_not_le h₁
       have heq : x % y = x := mod_eq_of_lt hgt
       rw [← heq] at hgt
       exact hgt
@@ -100,21 +100,21 @@ theorem mod_lt (x : Nat) {y : Nat} : y > 0 → x % y < y := by
     exact h₂ h₃
 
 theorem mod_le (x y : Nat) : x % y ≤ x := by
-  match Nat.ltOrGe x y with
-  | Or.inl h₁ => rw [mod_eq_of_lt h₁]; apply Nat.leRefl
-  | Or.inr h₁ => match eqZeroOrPos y with
-    | Or.inl h₂ => rw [h₂, Nat.mod_zero x]; apply Nat.leRefl
-    | Or.inr h₂ => exact Nat.leTrans (Nat.leOfLt (mod_lt _ h₂)) h₁
+  match Nat.lt_or_ge x y with
+  | Or.inl h₁ => rw [mod_eq_of_lt h₁]; apply Nat.le_refl
+  | Or.inr h₁ => match eq_zero_or_pos y with
+    | Or.inl h₂ => rw [h₂, Nat.mod_zero x]; apply Nat.le_refl
+    | Or.inr h₂ => exact Nat.le_trans (Nat.le_of_lt (mod_lt _ h₂)) h₁
 
 @[simp] theorem zero_mod (b : Nat) : 0 % b = 0 := by
   rw [mod_eq]
   have : ¬ (0 < b ∧ b ≤ 0) := by
     intro ⟨h₁, h₂⟩
-    exact absurd (Nat.ltOfLtOfLe h₁ h₂) (Nat.ltIrrefl 0)
+    exact absurd (Nat.lt_of_lt_of_le h₁ h₂) (Nat.lt_irrefl 0)
   simp [this]
 
 @[simp] theorem mod_self (n : Nat) : n % n = 0 := by
-  rw [mod_eq_sub_mod (Nat.leRefl _), Nat.sub_self, zero_mod]
+  rw [mod_eq_sub_mod (Nat.le_refl _), Nat.sub_self, zero_mod]
 
 theorem mod_one (x : Nat) : x % 1 = 0 := by
   have h : x % 1 < 1 := mod_lt x (by decide)
@@ -122,7 +122,7 @@ theorem mod_one (x : Nat) : x % 1 = 0 := by
     intro y
     cases y with
     | zero   => intro h; rfl
-    | succ y => intro h; apply absurd (Nat.lt_of_succ_lt_succ h) (Nat.notLtZero y)
+    | succ y => intro h; apply absurd (Nat.lt_of_succ_lt_succ h) (Nat.not_lt_zero y)
   exact this _ h
 
 end Nat
