stage0/src/Init/Data/Nat/Gcd.lean
@@ -11,7 +11,7 @@ namespace Nat
 private def gcdF (x : Nat) : (∀ x₁, x₁ < x → Nat → Nat) → Nat → Nat :=
   match x with
   | 0      => fun _ y => y
-  | succ x => fun f y => f (y % succ x) (mod_lt _ (zeroLtSucc  _)) (succ x)
+  | succ x => fun f y => f (y % succ x) (mod_lt _ (zero_lt_succ  _)) (succ x)
 
 @[extern "lean_nat_gcd"]
 def gcd (a b : @& Nat) : Nat :=
